src/PushButtonSynthesis/BaseConversion.v
@@ -97,6 +97,7 @@ Section __.
           {should_split_multiret : should_split_multiret_opt}
           {unfold_value_barrier : unfold_value_barrier_opt}
           {assembly_hints_lines : assembly_hints_lines_opt}
+          {ignore_unique_asm_names : ignore_unique_asm_names_opt}
           {widen_carry : widen_carry_opt}
           {widen_bytes : widen_bytes_opt}
           {assembly_calling_registers : assembly_calling_registers_opt}
